significant overhaul of X64.Memory.{fst, fsti} and Interop.fsti

vale/code/arch/x64/Interop.fsti
@@ -1,5 +1,5 @@
 module Interop
-
+module IB = Interop.Base
 module List = FStar.List.Tot.Base
 module HS = FStar.Monotonic.HyperStack
 module HH = FStar.Monotonic.HyperHeap
@@ -43,104 +43,77 @@ unfold
 let disjoint (#a:Type0) (ptr1 ptr2:B.buffer a) = M.loc_disjoint (M.loc_buffer ptr1) (M.loc_buffer ptr2)
 
 unfold
-let disjoint_or_eq ptr1 ptr2 = disjoint ptr1 ptr2 \/ ptr1 == ptr2
-
-let list_disjoint_or_eq (#a:Type0) (ptrs:list (B.buffer a)) =
-  forall p1 p2. List.memP p1 ptrs /\ List.memP p2 ptrs ==> disjoint_or_eq p1 p2
-
-let disjoint_addr addr1 length1 addr2 length2 =
-  (* The first buffer is completely before the second, or the opposite *)
-  addr1 + length1 < addr2 || addr2 + length2 < addr1
-
-type addr_map = (m:(b8 -> nat64){
-  (forall (buf1 buf2:b8).{:pattern (m buf1); (m buf2)} disjoint buf1 buf2 ==> 
-    disjoint_addr (m buf1) (B.length buf1) (m buf2) (B.length buf2)) /\
-  (forall (b:b8).{:pattern (m b)} m b + B.length b < pow2_64)})
+let disjoint_or_eq ptr1 ptr2 = IB.disjoint_or_eq_b8 ptr1 ptr2
 
 unfold
-let list_live (#a:Type0) mem (ptrs:list (B.buffer a)) = forall p . List.memP p ptrs ==> B.live mem p
+let list_disjoint_or_eq = IB.list_disjoint_or_eq
 
-let correct_down_p (mem:HS.mem) (addrs:addr_map) (heap:heap) (p:b8) =
-  let length = B.length p in
-  let contents = B.as_seq mem p in
-  let addr = addrs p in
-  (forall i.  0 <= i /\ i < length ==> heap.[addr + i] == UInt8.v (FStar.Seq.index contents i))
+unfold
+let disjoint_addr = IB.disjoint_addr
 
-val addrs_set: (ptrs:list b8) -> (addrs:addr_map) -> GTot (s:Set.set int{
-  forall x.{:pattern (Set.mem x s)} not (Set.mem x s) <==> 
-    (forall (b:b8{List.memP b ptrs}).{:pattern (addrs b)} x < addrs b \/ x >= addrs b + B.length b)})
-    
-val addrs_set_lemma: (ptrs1:list b8) -> (ptrs2:list b8) ->
-  (addrs:addr_map) -> Lemma
-  (requires forall b. List.memP b ptrs1 <==> List.memP b ptrs2)
-  (ensures addrs_set ptrs1 addrs == addrs_set ptrs2 addrs)
+type addr_map = IB.addr_map
 
-val addrs_set_concat: (ptrs:list b8) -> (a:b8) ->
-  (addrs:addr_map) -> Lemma
-  (addrs_set (a::ptrs) addrs == Set.union (addrs_set ptrs addrs) (addrs_set [a] addrs))
+unfold
+let list_live = IB.list_live
+
+let valid_addr (mem:IB.mem) (x:int) = Set.mem x (IB.addrs_set mem)
+
+val addrs_set_lemma (mem:IB.mem) (x:int)
+  : Lemma (let addrs = IB.addrs_of_mem mem in
+           let ptrs = IB.ptrs_of_mem mem in
+           valid_addr mem x <==>
+           (exists (b:b8{List.memP b ptrs}).{:pattern (addrs b)} addrs b <= x /\ x < addrs b + B.length b))
+          [SMTPat (Set.mem x (IB.addrs_set mem))]
   
-val addrs_set_mem: (ptrs:list b8) -> (a:b8) ->
-  (addrs:addr_map) -> (i:int) -> Lemma
-  (requires List.memP a ptrs /\ i >= addrs a /\ i < addrs a + B.length a)
-  (ensures Set.mem i (addrs_set ptrs addrs))
+let addrs_set_mem (mem:IB.mem) (a:b8) (i:int)
+  : Lemma
+    (requires (let ptrs = IB.ptrs_of_mem mem in
+               let addrs = IB.addrs_of_mem mem in
+               List.memP a ptrs /\ i >= addrs a /\ i < addrs a + B.length a))
+    (ensures valid_addr mem i)
+  = ()
   
-let correct_down mem (addrs:addr_map) (ptrs: list b8) heap =
-  Set.equal (addrs_set ptrs addrs) (Map.domain heap) /\ 
-  (forall p. List.memP p ptrs ==> correct_down_p mem addrs heap p)
-
 (* Takes a Low* Hyperstack and a list of buffers and create a vale memory + keep track of the vale addresses *)
-val down_mem: (mem:HS.mem) -> (addrs: addr_map) -> (ptrs:list b8{list_disjoint_or_eq ptrs}) -> GTot (heap :heap {correct_down mem addrs ptrs heap})
+val down_mem: IB.down_mem_t
 
 val same_unspecified_down: 
-  (mem1: HS.mem) -> 
-  (mem2: HS.mem) -> 
-  (addrs:addr_map) ->
-  (ptrs:list b8{list_disjoint_or_eq ptrs}) ->
+  (hs1: HS.mem) -> 
+  (hs2: HS.mem) -> 
+  (ptrs:list b8{list_disjoint_or_eq ptrs /\ list_live hs1 ptrs /\ list_live hs2 ptrs}) ->
   Lemma (
-    let heap1 = down_mem mem1 addrs ptrs in
-    let heap2 = down_mem mem2 addrs ptrs in
-    forall i. (forall (b:b8{List.memP b ptrs}). 
-      let base = addrs b in
-      i < base \/ i >= base + B.length b) ==>
-      heap1.[i] == heap2.[i])
+    let mem1 = IB.mem_of_hs_roots ptrs hs1 in
+    let mem2 = IB.mem_of_hs_roots ptrs hs2 in
+    let addrs = IB.addrs_of_mem mem1 in
+    let heap1 = down_mem mem1 in
+    let heap2 = down_mem mem2 in
+    forall i. not (valid_addr mem1 i) ==>
+         heap1.[i] == heap2.[i])
 
-let get_seq_heap (heap:heap) (addrs:addr_map) (b:b8) : GTot (Seq.lseq UInt8.t (B.length b)) =
-  let length = B.length b in
-  let contents (i:nat{i < length}) = UInt8.uint_to_t heap.[addrs b + i] in
-  Seq.init length contents
+let get_seq_heap (heap:heap) (addrs:addr_map) (b:b8) 
+  : GTot (Seq.lseq UInt8.t (B.length b)) 
+  = let length = B.length b in
+    let contents (i:nat{i < length}) = UInt8.uint_to_t heap.[addrs b + i] in
+    Seq.init length contents
 
-val up_mem: 
-  (heap:heap) -> 
-  (addrs:addr_map) -> 
-  (ptrs: list b8{list_disjoint_or_eq ptrs}) -> 
-  (mem:HS.mem{list_live mem ptrs /\ Set.equal (addrs_set ptrs addrs) (Map.domain heap)}) -> 
-  GTot (new_mem:HS.mem{correct_down new_mem addrs ptrs heap /\ list_live new_mem ptrs})
+val up_mem (heap:heap) (mem:IB.mem{Set.equal (IB.addrs_set mem) (Map.domain heap)})
+  : GTot (new_mem:IB.mem{IB.ptrs_of_mem mem == IB.ptrs_of_mem mem /\
+                         IB.correct_down new_mem heap})
 
-val down_up_identity: 
-  (mem:HS.mem) -> 
-  (addrs:addr_map) -> 
-  (ptrs:list b8{list_disjoint_or_eq ptrs /\ list_live mem ptrs }) -> 
-  Lemma (
-    let heap = down_mem mem addrs ptrs in 
-    let new_mem = up_mem heap addrs ptrs mem in
-    mem == new_mem)
+val down_up_identity (mem:IB.mem)
+  : Lemma (mem == up_mem (down_mem mem) mem)
 
-val up_down_identity:
-  (mem:HS.mem) ->
-  (addrs:addr_map) ->
-  (ptrs:list b8{list_disjoint_or_eq ptrs /\ list_live mem ptrs}) ->
-  (heap:heap{Set.equal (addrs_set ptrs addrs) (Map.domain heap)}) -> 
-  Lemma
-    (requires (forall x. not (Map.contains heap x) ==> Map.sel heap x == Map.sel (down_mem mem addrs ptrs) x))
-    (ensures (down_mem (up_mem heap addrs ptrs mem) addrs ptrs == heap))
+val up_down_identity (mem:IB.mem)
+                     (heap:heap{Set.equal (IB.addrs_set mem) (Map.domain heap)})
+  : Lemma
+      (requires (forall x. not (Map.contains heap x) ==> Map.sel heap x == Map.sel (down_mem mem) x))
+      (ensures (down_mem (up_mem heap mem) == heap))
 
-val update_buffer_up_mem:
-  (ptrs:list b8{list_disjoint_or_eq ptrs}) ->
-  (addrs:addr_map) ->
-  (mem:HS.mem{list_live mem ptrs}) ->
-  (b:b8{List.memP b ptrs}) ->
-  (heap1:heap{correct_down mem addrs ptrs heap1}) ->
-  (heap2:heap{Set.equal (Map.domain heap1) (Map.domain heap2)}) -> Lemma
-  (requires (forall x. x < addrs b \/ x >= addrs b + B.length b ==> heap1.[x] == heap2.[x]))
-  (ensures up_mem heap2 addrs ptrs mem == 
-    B.g_upd_seq b (get_seq_heap heap2 addrs b) mem)
+val update_buffer_up_mem
+      (mem:IB.mem)
+      (b:b8{List.memP b (IB.ptrs_of_mem mem)})
+      (heap1:heap{IB.correct_down mem heap1})
+      (heap2:heap{Set.equal (Map.domain heap1) (Map.domain heap2)})
+ : Lemma
+      (requires (forall x. not (valid_addr mem x) ==> heap1.[x] == heap2.[x]))
+      (ensures IB.hs_of_mem (up_mem heap2 mem) ==
+               B.g_upd_seq b (get_seq_heap heap2 (IB.addrs_of_mem mem) b) (IB.hs_of_mem mem))
