vale/code/arch/x64/X64.Memory.fst
@@ -1,5 +1,6 @@
 module X64.Memory
-
+open Interop.Base
+module IB = Interop.Base
 module I = Interop
 module HS = FStar.HyperStack
 module B = LowStar.Buffer
@@ -11,17 +12,10 @@ module S = X64.Bytes_Semantics_s
 
 #reset-options "--initial_fuel 2 --max_fuel 2 --initial_ifuel 1 --max_ifuel 1"
 
-let b8 = B.buffer UInt8.t
+let b8 = IB.b8
 
 let heap = H.heap
-noeq type mem' = {
-  addrs : I.addr_map;
-  ptrs : list b8;
-  hs : HS.mem;
-  }
-
-type mem = (m:mem'{I.list_disjoint_or_eq #UInt8.t m.ptrs /\
-  I.list_live m.hs m.ptrs})
+type mem = IB.mem
 
 let op_String_Access = Map.sel
 let op_String_Assignment = Map.upd
@@ -33,53 +27,32 @@ let tuint16 = UInt16.t
 let tuint32 = UInt32.t
 let tuint64 = UInt64.t
 
-let m_of_typ (t:typ) : Type0 =
+let v_of_typ (t:base_typ) (v:base_typ_as_vale_type t) : base_typ_as_type t =
   match t with
-  | TBase TUInt8 -> tuint8
-  | TBase TUInt16 -> tuint16
-  | TBase TUInt32 -> tuint32
-  | TBase TUInt64 -> tuint64
-  | TBase TUInt128 -> quad32
+  | TUInt8 -> UInt8.uint_to_t v
+  | TUInt16 -> UInt16.uint_to_t v
+  | TUInt32 -> UInt32.uint_to_t v
+  | TUInt64 -> UInt64.uint_to_t v
+  | TUInt128 -> v
 
-let v_of_typ (t:typ) (v:type_of_typ t) :  (m_of_typ t) =
+let v_to_typ (t:base_typ) (v:base_typ_as_type t) : base_typ_as_vale_type t =
   match t with
-  | TBase TUInt8 -> coerce ((m_of_typ t)) (UInt8.uint_to_t v)
-  | TBase TUInt16 -> coerce ((m_of_typ t)) (UInt16.uint_to_t v)
-  | TBase TUInt32 -> coerce ((m_of_typ t)) (UInt32.uint_to_t v)
-  | TBase TUInt64 -> coerce ((m_of_typ t)) (UInt64.uint_to_t v)
-  | TBase TUInt128 -> v
+  | TUInt8 -> UInt8.v v
+  | TUInt16 -> UInt16.v v
+  | TUInt32 -> UInt32.v v
+  | TUInt64 -> UInt64.v v
+  | TUInt128 -> v
 
-let v_to_typ (t:typ) (v:(m_of_typ t)) : type_of_typ t =
-  match t with
-  | TBase TUInt8 -> UInt8.v (coerce UInt8.t v)
-  | TBase TUInt16 -> UInt16.v (coerce UInt16.t v)
-  | TBase TUInt32 -> UInt32.v (coerce UInt32.t v)
-  | TBase TUInt64 -> UInt64.v (coerce UInt64.t v)
-  | TBase TUInt128 -> v
-
-let lemma_v_to_of_typ (t:typ) (v:type_of_typ t) : Lemma
+let lemma_v_to_of_typ (t:base_typ) (v:base_typ_as_vale_type t) : Lemma
   (ensures v_to_typ t (v_of_typ t v) == v)
   [SMTPat (v_to_typ t (v_of_typ t v))]
-  =
-  match t with
-  | TBase TUInt8 -> assert (UInt8.v (UInt8.uint_to_t v) == v)
-  | TBase TUInt16 -> assert (UInt16.v (UInt16.uint_to_t v) == v)
-  | TBase TUInt32 -> assert (UInt32.v (UInt32.uint_to_t v) == v)
-  | TBase TUInt64 -> assert (UInt64.v (UInt64.uint_to_t v) == v)
-  | TBase TUInt128 -> ()
+  = ()
 
-let view_n = function
-  | TBase TUInt8 -> 1
-  | TBase TUInt16 -> 2
-  | TBase TUInt32 -> 4
-  | TBase TUInt64 -> 8
-  | TBase TUInt128 -> 16
-
-val uint8_view: (v:BV.view UInt8.t UInt8.t{BV.View?.n v == view_n (TBase TUInt8)})
-val uint16_view: (v:BV.view UInt8.t UInt16.t{BV.View?.n v == view_n (TBase TUInt16)})
-val uint32_view: (v:BV.view UInt8.t UInt32.t{BV.View?.n v == view_n (TBase TUInt32)})
-val uint64_view: (v:BV.view UInt8.t UInt64.t{BV.View?.n v == view_n (TBase TUInt64)})
-val uint128_view: (v:BV.view UInt8.t quad32{BV.View?.n v == view_n (TBase TUInt128)})
+// val uint8_view: (v:BV.view UInt8.t UInt8.t{BV.View?.n v == view_n (TUInt8)})
+// val uint16_view: (v:BV.view UInt8.t UInt16.t{BV.View?.n v == view_n (TUInt16)})
+// val uint32_view: (v:BV.view UInt8.t UInt32.t{BV.View?.n v == view_n (TUInt32)})
+// val uint64_view: (v:BV.view UInt8.t UInt64.t{BV.View?.n v == view_n (TUInt64)})
+// val uint128_view: (v:BV.view UInt8.t quad32{BV.View?.n v == view_n (TUInt128)})
 
 let uint8_view = Views.view8
 let uint16_view = Views.view16
@@ -87,24 +60,24 @@ let uint32_view = Views.view32
 let uint64_view = Views.view64
 let uint128_view = Views.view128
 
-val uint_view (t:typ) : (v:BV.view UInt8.t (m_of_typ t){BV.View?.n v == view_n t})
+val uint_view (t:base_typ) : (v:BV.view UInt8.t (IB.base_typ_as_type t){BV.View?.n v == view_n t})
 
 let uint_view = function
-  | TBase TUInt8 -> uint8_view
-  | TBase TUInt16 -> uint16_view
-  | TBase TUInt32 -> uint32_view
-  | TBase TUInt64 -> uint64_view
-  | TBase TUInt128 -> uint128_view
+  | TUInt8 -> uint8_view
+  | TUInt16 -> uint16_view
+  | TUInt32 -> uint32_view
+  | TUInt64 -> uint64_view
+  | TUInt128 -> uint128_view
 
-let buffer t = (b:b8{B.length b % view_n t == 0})
+let buffer = IB.buf_t
 
 let buffer_as_seq #t h b =
-  let s = BV.as_seq h.hs (BV.mk_buffer_view b (uint_view t)) in
+  let s = BV.as_seq (IB.hs_of_mem h) (BV.mk_buffer_view b (uint_view t)) in
   let len = Seq.length s in
-  let contents (i:nat{i < len}) : type_of_typ t = v_to_typ t (Seq.index s i) in
+  let contents (i:nat{i < len}) : base_typ_as_vale_type t = v_to_typ t (Seq.index s i) in
   Seq.init len contents
 
-let buffer_readable #t h b = List.memP b h.ptrs
+let buffer_readable #t h b = List.memP b (IB.ptrs_of_mem h)
 let buffer_length #t b = BV.length (BV.mk_buffer_view b (uint_view t))
 let loc = M.loc
 let loc_none = M.loc_none
@@ -112,19 +85,17 @@ let loc_union = M.loc_union
 let loc_buffer #t b = M.loc_buffer b
 let loc_disjoint = M.loc_disjoint
 let loc_includes = M.loc_includes
-let modifies s h h' =
-  M.modifies s h.hs h'.hs /\ h.ptrs == h'.ptrs /\ h.addrs == h'.addrs
+let modifies s h h' = M.modifies s h.hs h'.hs /\ h.ptrs == h'.ptrs /\ h.addrs == h'.addrs
 
 
-let buffer_addr #t b h =
-  let addrs = h.addrs in
-  addrs b
-
+let buffer_addr #t b h = IB.addrs_of_mem h b
+open FStar.Mul
 val index64_get_heap_val64 (h:mem)
                            (b:buffer64{List.memP b h.ptrs})
-                           (heap:S.heap{I.correct_down h.hs h.addrs h.ptrs heap})
-                           (i:nat{i < buffer_length b}) : Lemma
-(Seq.index (buffer_as_seq h b) i == S.get_heap_val64 (buffer_addr b h + 8 `op_Multiply` i) heap)
+                           (heap:S.heap{IB.correct_down h heap})
+                           (i:nat{i < buffer_length b})
+   : Lemma (Seq.index (buffer_as_seq h b) i ==
+            S.get_heap_val64 (buffer_addr b h + 8 * i) heap)
 
 #set-options "--z3rlimit 20"
 
@@ -140,15 +111,17 @@ let index_helper (x y:int) (heap:S.heap) : Lemma
   (ensures heap.[x] == heap.[y]) = ()
 
 let index_mul_helper (addr i n j:int) : Lemma
-  (addr + (i `op_Multiply` n + j) == addr + n `op_Multiply` i + j) =
+  (addr + (i * n + j) == addr + n * i + j) =
  ()
+
+#set-options "--max_fuel 0 --max_ifuel 0"
 
 let index64_get_heap_val64 h b heap i =
   let open FStar.Mul in
   let vb = BV.mk_buffer_view b uint64_view in
   let ptr = buffer_addr b h + 8 * i in
   let s = B.as_seq h.hs b in
-  let t = TBase TUInt64 in
+  let t = TUInt64 in
   let addr = buffer_addr b h in
   BV.length_eq vb;
   BV.view_indexing vb i;
@@ -171,15 +144,15 @@ open Words_s
 
 val index128_get_heap_val128 (h:mem)
                            (b:buffer128{List.memP b h.ptrs})
-                           (heap:S.heap{I.correct_down h.hs h.addrs h.ptrs heap})
+                           (heap:S.heap{IB.correct_down h heap})
                            (i:nat{i < buffer_length b}) : Lemma
 (let addr = buffer_addr b h in
  Seq.index (buffer_as_seq h b) i ==
   Mkfour
-    (S.get_heap_val32 (addr + 16 `op_Multiply` i) heap)
-    (S.get_heap_val32 (addr + 16 `op_Multiply` i+4) heap)
-    (S.get_heap_val32 (addr + 16 `op_Multiply` i+8) heap)
-    (S.get_heap_val32 (addr + 16 `op_Multiply` i +12) heap)
+    (S.get_heap_val32 (addr + 16 * i) heap)
+    (S.get_heap_val32 (addr + 16 * i+4) heap)
+    (S.get_heap_val32 (addr + 16 * i+8) heap)
+    (S.get_heap_val32 (addr + 16 * i +12) heap)
  )
 
 #set-options "--z3rlimit 50"
@@ -226,7 +199,7 @@ let lemma_modifies_goal_directed s h1 h2 = ()
 
 let buffer_length_buffer_as_seq #t h b = ()
 
-val same_underlying_seq (#t:typ) (h1 h2:mem) (b:buffer t) : Lemma
+val same_underlying_seq (#t:base_typ) (h1 h2:mem) (b:buffer t) : Lemma
   (requires Seq.equal (B.as_seq h1.hs b) (B.as_seq h2.hs b))
   (ensures Seq.equal (buffer_as_seq h1 b) (buffer_as_seq h2 b))
 
@@ -279,13 +252,14 @@ let modifies_goal_directed_trans s12 h1 h2 s13 h3 =
 
 let modifies_goal_directed_trans2 s12 h1 h2 s13 h3 = modifies_goal_directed_trans s12 h1 h2 s13 h3
 
-let default_of_typ (t:typ) : type_of_typ t =
+let default_of_typ (t:base_typ) : base_typ_as_vale_type t =
+  allow_inversion base_typ;
   match t with
-  | TBase TUInt8 -> 0
-  | TBase TUInt16 -> 0
-  | TBase TUInt32 -> 0
-  | TBase TUInt64 -> 0
-  | TBase TUInt128 -> Words_s.Mkfour #nat32 0 0 0 0
+  | TUInt8 -> 0
+  | TUInt16 -> 0
+  | TUInt32 -> 0
+  | TUInt64 -> 0
+  | TUInt128 -> Words_s.Mkfour #nat32 0 0 0 0
 
 let buffer_read #t b i h =
   if i < 0 || i >= buffer_length b then default_of_typ t else
@@ -326,325 +300,278 @@ let buffer_write #t b i v h =
    BV.as_buffer_mk_buffer_view b view;
    BV.upd_modifies h.hs bv i (v_of_typ t v);
    let hs' = BV.upd h.hs bv i (v_of_typ t v) in
-   let h':mem = {h with hs = hs'} in
+   let h':mem = Mem h.ptrs h.addrs hs' in
    seq_upd h.hs bv i (v_of_typ t v);
    assert (Seq.equal (buffer_as_seq h' b) (Seq.upd (buffer_as_seq h b) i v));
    h'
  end
 
-val addr_in_ptr: (#t:typ) -> (addr:int) -> (ptr:buffer t) -> (h:mem) ->
+val addr_in_ptr: (#t:base_typ) -> (addr:int) -> (ptr:buffer t) -> (h:mem) ->
   GTot (b:bool{ not b <==> (forall i. 0 <= i /\ i < buffer_length ptr ==>
-    addr <> (buffer_addr ptr h) + (view_n t) `op_Multiply` i)})
+    addr <> (buffer_addr ptr h) + (view_n t) * i)})
 
 // Checks if address addr corresponds to one of the elements of buffer ptr
 let addr_in_ptr #t addr ptr h =
   let n = buffer_length ptr in
   let base = buffer_addr ptr h in
   let rec aux (i:nat) : Tot (b:bool{not b <==> (forall j. i <= j /\ j < n ==>
-    addr <> base + (view_n t) `op_Multiply` j)})
+    addr <> base + (view_n t) * j)})
     (decreases %[n-i]) =
     if i >= n then false
-    else if addr = base + (view_n t) `op_Multiply` i then true
+    else if addr = base + (view_n t) * i then true
     else aux (i+1)
   in aux 0
 
-let rec get_addr_in_ptr (t:typ) (n base addr:nat) (i:nat{exists j. i <= j /\ j < n /\ base + (view_n t) `op_Multiply` j == addr}) :
-    GTot (j:nat{base + (view_n t) `op_Multiply` j == addr})
+let valid_offset (t:base_typ) (n base addr i:nat) = exists j. i <= j /\ j < n /\ base + (view_n t) * j == addr
+
+let rec get_addr_in_ptr (t:base_typ) (n base addr:nat) (i:nat{valid_offset t n base addr i})
+  : GTot (j:nat{base + (view_n t) * j == addr})
     (decreases %[n-i]) =
-    if base + (view_n t) `op_Multiply` i = addr then i
-    else if i >= n then i
+    if base + (view_n t) * i = addr then i
     else get_addr_in_ptr t n base addr (i+1)
 
-let valid_buffer (t:typ) (addr:int) (b:b8) (h:mem) : GTot bool = B.length b % (view_n t) = 0 && (addr_in_ptr #t addr b h)
+let valid_buffer (t:base_typ) (addr:int) (b:b8) (h:mem) : GTot bool =
+  B.length b % (view_n t) = 0 &&
+  addr_in_ptr #t addr b h
 
-let rec valid_mem_aux (t:typ) addr (ps:list b8) (h:mem) : GTot (b:bool{
-  (not b) <==> (forall (x:buffer t). (List.memP x ps ==> not (valid_buffer t addr x h) ))})
+#set-options "--max_fuel 1 --max_ifuel 1"
+let sub_list (p1 p2:list 'a) = forall x. {:pattern List.memP x p2} List.memP x p1 ==> List.memP x p2
+
+let rec valid_mem_aux (t:base_typ) addr (ps:list b8) (h:mem {sub_list ps h.ptrs})
+  : GTot (b:bool{
+           b <==>
+           (exists (x:buffer t). {:pattern (List.memP x ps) \/ (valid_buffer t addr x h)}
+             List.memP x ps /\ valid_buffer t addr x h)})
   = match ps with
     | [] -> false
-    | a::q -> if valid_buffer t addr a h then true else valid_mem_aux t addr q h
+    | a::q -> valid_buffer t addr a h || valid_mem_aux t addr q h
+let valid_mem (t:base_typ) addr (h:mem) = valid_mem_aux t addr h.ptrs h
+let valid_mem64 ptr h = valid_mem (TUInt64) ptr h
 
-let valid_mem64 ptr h = valid_mem_aux (TBase TUInt64) ptr h.ptrs h
+let rec find_valid_buffer_aux (t:base_typ) (addr:int) (ps:list b8) (h:mem{sub_list ps h.ptrs})
+  : GTot (o:option (buffer t){
+    match o with
+    | None -> not (valid_mem_aux t addr ps h)
+    | Some a -> valid_buffer t addr a h /\ List.memP a ps})
+  = match ps with
+    | [] -> None
+    | a::q -> if valid_buffer t addr a h then Some a else find_valid_buffer_aux t addr q h
+let find_valid_buffer (t:base_typ) (addr:int) (h:mem) = find_valid_buffer_aux t addr h.ptrs h
+let rec find_valid_buffer_aux_ps (t:base_typ) (addr:int) (ps:list b8) (h1:mem) (h2:mem{h1.ptrs == h2.ptrs /\ sub_list ps h1.ptrs})
+  : Lemma (find_valid_buffer_aux t addr ps h1 == find_valid_buffer_aux t addr ps h2)
+  = match ps with
+    | [] -> ()
+    | a::q -> find_valid_buffer_aux_ps t addr q h1 h2
+let find_valid_buffer_ps (t:base_typ) (addr:int) (h1:mem) (h2:mem{h1.ptrs==h2.ptrs})
+  : Lemma (find_valid_buffer t addr h1 == find_valid_buffer t addr h2)
+  = find_valid_buffer_aux_ps t addr h1.ptrs h1 h2
+let find_valid_buffer_valid_offset (t:base_typ) (addr:int) (h:mem)
+  : Lemma (match find_valid_buffer t addr h with
+           | None -> True
+           | Some a ->
+             let base = buffer_addr a h in
+             valid_offset t (buffer_length a) base addr 0)
+  = ()
 
-let rec load_mem_aux (t:typ) addr (ps:list b8) (h:mem{forall x. List.memP x ps ==> List.memP x h.ptrs }) :
-  GTot (type_of_typ t) =
-  match ps with
-  | [] -> default_of_typ t
-  | a::q ->
-    if valid_buffer t addr a h then
-    begin
-      let a:buffer t = a in
-      let base = buffer_addr a h in
-      buffer_read a (get_addr_in_ptr t (buffer_length a) base addr 0) h
-    end
-    else load_mem_aux t addr q h
+let load_mem (t:base_typ) addr (h:mem)
+  : GTot (base_typ_as_vale_type t) =
+  match find_valid_buffer t addr h with
+  | None -> default_of_typ t
+  | Some a ->
+    let base = buffer_addr a h in
+    buffer_read a (get_addr_in_ptr t (buffer_length a) base addr 0) h
 
 let load_mem64 ptr h =
   if not (valid_mem64 ptr h) then 0
-  else load_mem_aux (TBase TUInt64) ptr h.ptrs h
+  else load_mem (TUInt64) ptr h
 
-let length_t_eq (t:typ) (b:buffer t) : Lemma (B.length b == buffer_length b `op_Multiply` (view_n t)) =
+let length_t_eq (t:base_typ) (b:buffer t) : Lemma (B.length b == buffer_length b * (view_n t)) =
   BV.as_buffer_mk_buffer_view b (uint_view t);
   BV.get_view_mk_buffer_view b (uint_view t);
   BV.length_eq (BV.mk_buffer_view b (uint_view t))
 
-let rec get_addr_ptr (t:typ) (ptr:int) (h:mem) (ps:list b8{valid_mem_aux t ptr ps h}) :
-  GTot (b:buffer t{List.memP b ps /\ valid_buffer t ptr b h}) =
-  match ps with
-  // The list cannot be empty because of the mem predicate
-  | a::q -> if valid_buffer t ptr a h then a else get_addr_ptr t ptr h q
+let get_addr_ptr (t:base_typ) (ptr:int) (h:mem{valid_mem t ptr h})
+  : GTot (b:buffer t{List.memP b h.ptrs /\ valid_buffer t ptr b h})
+  = Some?.v (find_valid_buffer t ptr h)
 
-#set-options "--z3rlimit 100"
+#reset-options "--max_fuel 0 --max_ifuel 0 --initial_fuel 0 --initial_ifuel 0"
+val load_buffer_read
+          (t:base_typ)
+          (ptr:int)
+          (h:mem{valid_mem t ptr h})
+ : Lemma
+    (ensures (let b = get_addr_ptr t ptr h in
+              let i = get_addr_in_ptr t (buffer_length b) (buffer_addr b h) ptr 0 in
+              load_mem t ptr h == buffer_read #t b i h))
+let load_buffer_read t ptr h = ()
 
-let rec load_buffer_read (t:typ) (ptr:int) (h:mem)
-  (ps:list b8{I.list_disjoint_or_eq ps /\ valid_mem_aux t ptr ps h /\
-    (forall x. List.memP x ps ==> List.memP x h.ptrs)}) : Lemma
-  (let b = get_addr_ptr t ptr h ps in
-   length_t_eq t b;
-   let i = get_addr_in_ptr t (buffer_length b) (buffer_addr b h) ptr 0 in
-   load_mem_aux t ptr ps h == buffer_read #t b i h) =
-      match ps with
-      | a::q ->
-        if valid_buffer t ptr a h then () else load_buffer_read t ptr h q
-
-let rec store_mem_aux (t:typ) addr (ps:list b8) (v:type_of_typ t) (h:mem{forall x. List.memP x ps ==> List.memP x h.ptrs }) :
-  GTot (h1:mem{h.addrs == h1.addrs /\ h.ptrs == h1.ptrs }) =
-  match ps with
-  | [] -> h
-  | a::q ->
-    if valid_buffer t addr a h then
-    begin
-      let a:buffer t = a in
+let store_mem (t:base_typ) addr (v:base_typ_as_vale_type t) (h:mem)
+  : GTot (h1:mem{h.addrs == h1.addrs /\ h.ptrs == h1.ptrs })
+  = match find_valid_buffer t addr h with
+    | None -> h
+    | Some a ->
       let base = buffer_addr a h in
       buffer_write a (get_addr_in_ptr t (buffer_length a) base addr 0) v h
-    end
-    else store_mem_aux t addr q v h
 
 let store_mem64 i v h =
   if not (valid_mem64 i h) then h
-  else store_mem_aux (TBase TUInt64) i h.ptrs v h
+  else store_mem (TUInt64) i v h
 
-let rec store_buffer_write (t:typ) (ptr:int) (v:type_of_typ t) (h:mem)
-  (ps:list b8{I.list_disjoint_or_eq ps /\ valid_mem_aux t ptr ps h /\
-    (forall x. List.memP x ps ==> List.memP x h.ptrs)}) : Lemma
-  (let b = get_addr_ptr t ptr h ps in
-   length_t_eq t b;
-   let i = get_addr_in_ptr t (buffer_length b) (buffer_addr b h) ptr 0 in
-   store_mem_aux t ptr ps v h == buffer_write b i v h) =
-      match ps with
-      | a::q ->
-        if valid_buffer t ptr a h then () else store_buffer_write t ptr v h q
+val store_buffer_write
+          (t:base_typ)
+          (ptr:int)
+          (v:base_typ_as_vale_type t)
+          (h:mem{valid_mem t ptr h})
+  : Lemma
+      (let b = get_addr_ptr t ptr h in
+       let i = get_addr_in_ptr t (buffer_length b) (buffer_addr b h) ptr 0 in
+       store_mem t ptr v h == buffer_write b i v h)
+let store_buffer_write t ptr v h = ()
 
-let valid_mem128 ptr h = valid_mem_aux (TBase TUInt128) ptr h.ptrs h
+let valid_mem128 ptr h = valid_mem_aux (TUInt128) ptr h.ptrs h
 let load_mem128 ptr h =
-  if not (valid_mem128 ptr h) then (default_of_typ (TBase TUInt128))
-  else load_mem_aux (TBase TUInt128) ptr h.ptrs h
+  if not (valid_mem128 ptr h) then (default_of_typ (TUInt128))
+  else load_mem (TUInt128) ptr h
 let store_mem128 ptr v h =
   if not (valid_mem128 ptr h) then h
-  else store_mem_aux (TBase TUInt128) ptr h.ptrs v h
+  else store_mem (TUInt128) ptr v h
 
 let lemma_valid_mem64 b i h = ()
 
-#set-options "--z3rlimit 20"
-
 let lemma_load_mem64 b i h =
-  let addr = buffer_addr b h + 8 `op_Multiply` i in
+  let addr = buffer_addr b h + 8 * i in
   lemma_valid_mem64 b i h;
-  let rec aux (ps:list b8{I.list_disjoint_or_eq ps})
-    (h0:mem{h == h0 /\ (forall x. List.memP x ps ==> List.memP x h0.ptrs)}) :
-    Lemma (requires (List.memP b ps /\ i < buffer_length b) )
-    (ensures (load_mem_aux (TBase TUInt64) addr ps h0 == buffer_read b i h0)) =
-    match ps with
-    | [] -> ()
-    | a::q ->
-      if valid_buffer (TBase TUInt64) addr a h0 then begin
-        let a:buffer64 = a in
-        BV.length_eq (BV.mk_buffer_view a uint64_view);
-        BV.get_view_mk_buffer_view a uint64_view;
-        BV.as_buffer_mk_buffer_view a uint64_view;
-        BV.length_eq (BV.mk_buffer_view b uint64_view);
-        BV.get_view_mk_buffer_view b uint64_view;
-        BV.as_buffer_mk_buffer_view b uint64_view;
-
-        assert (I.disjoint_or_eq a b);
-        assert (a == b);
-          ()
-      end
-      else begin
-        assert (b =!= a);
-          aux q h0
-      end
-  in aux h.ptrs h
+  match find_valid_buffer TUInt64 addr h with
+  | None -> ()
+  | Some a ->
+    BV.length_eq (BV.mk_buffer_view a uint64_view);
+    BV.get_view_mk_buffer_view a uint64_view;
+    BV.as_buffer_mk_buffer_view a uint64_view;
+    BV.length_eq (BV.mk_buffer_view b uint64_view);
+    BV.get_view_mk_buffer_view b uint64_view;
+    BV.as_buffer_mk_buffer_view b uint64_view;
+    assert (I.disjoint_or_eq a b);
+    assert (a == b)
 
 let lemma_store_mem64 b i v h =
-  let addr = buffer_addr b h + 8 `op_Multiply` i in
+  let addr = buffer_addr b h + 8 * i in
   lemma_valid_mem64 b i h;
-  let rec aux (ps:list b8{I.list_disjoint_or_eq ps})
-    (h0:mem{h == h0 /\ (forall x. List.memP x ps ==> List.memP x h0.ptrs)}) :
-    Lemma (requires (List.memP b ps /\ i < buffer_length b) )
-    (ensures (store_mem_aux (TBase TUInt64) addr ps v h0 == buffer_write b i v h0)) =
-    match ps with
-    | [] -> ()
-    | a::q ->
-      if valid_buffer (TBase TUInt64) addr a h0 then begin
-        let a:buffer64 = a in
-        BV.length_eq (BV.mk_buffer_view a uint64_view);
-        BV.get_view_mk_buffer_view a uint64_view;
-        BV.as_buffer_mk_buffer_view a uint64_view;
-        BV.length_eq (BV.mk_buffer_view b uint64_view);
-        BV.get_view_mk_buffer_view b uint64_view;
-        BV.as_buffer_mk_buffer_view b uint64_view;
-
-        assert (I.disjoint_or_eq a b);
-        assert (a == b);
-          ()
-      end
-      else begin
-        assert (b =!= a);
-          aux q h0
-      end
-  in aux h.ptrs h
+  match find_valid_buffer TUInt64 addr h with
+  | None -> ()
+  | Some a ->
+    BV.length_eq (BV.mk_buffer_view a uint64_view);
+    BV.get_view_mk_buffer_view a uint64_view;
+    BV.as_buffer_mk_buffer_view a uint64_view;
+    BV.length_eq (BV.mk_buffer_view b uint64_view);
+    BV.get_view_mk_buffer_view b uint64_view;
+    BV.as_buffer_mk_buffer_view b uint64_view;
+    assert (I.disjoint_or_eq a b);
+    assert (a == b)
 
 let lemma_valid_mem128 b i h = ()
 
 let lemma_load_mem128 b i h =
-  let addr = buffer_addr b h + 16 `op_Multiply` i in
+  let addr = buffer_addr b h + 16 * i in
   lemma_valid_mem128 b i h;
-  let rec aux (ps:list b8{I.list_disjoint_or_eq ps})
-    (h0:mem{h == h0 /\ (forall x. List.memP x ps ==> List.memP x h0.ptrs)}) :
-    Lemma (requires (List.memP b ps /\ i < buffer_length b) )
-    (ensures (load_mem_aux (TBase TUInt128) addr ps h0 == buffer_read b i h0)) =
-    match ps with
-    | [] -> ()
-    | a::q ->
-      if valid_buffer (TBase TUInt128) addr a h0 then begin
-        let a:buffer128 = a in
-        BV.length_eq (BV.mk_buffer_view a uint128_view);
-        BV.get_view_mk_buffer_view a uint128_view;
-        BV.as_buffer_mk_buffer_view a uint128_view;
-        BV.length_eq (BV.mk_buffer_view b uint128_view);
-        BV.get_view_mk_buffer_view b uint128_view;
-        BV.as_buffer_mk_buffer_view b uint128_view;
-
-        assert (I.disjoint_or_eq a b);
-        assert (a == b);
-          ()
-      end
-      else begin
-        assert (b =!= a);
-          aux q h0
-      end
-  in aux h.ptrs h
+  match find_valid_buffer TUInt128 addr h with
+  | None -> ()
+  | Some a ->
+    BV.length_eq (BV.mk_buffer_view a uint128_view);
+    BV.get_view_mk_buffer_view a uint128_view;
+    BV.as_buffer_mk_buffer_view a uint128_view;
+    BV.length_eq (BV.mk_buffer_view b uint128_view);
+    BV.get_view_mk_buffer_view b uint128_view;
+    BV.as_buffer_mk_buffer_view b uint128_view;
+    assert (I.disjoint_or_eq a b);
+    assert (a == b)
 
 let lemma_store_mem128 b i v h =
-  let addr = buffer_addr b h + 16 `op_Multiply` i in
+  let addr = buffer_addr b h + 16 * i in
   lemma_valid_mem128 b i h;
-  let rec aux (ps:list b8{I.list_disjoint_or_eq ps})
-    (h0:mem{h == h0 /\ (forall x. List.memP x ps ==> List.memP x h0.ptrs)}) :
-    Lemma (requires (List.memP b ps /\ i < buffer_length b) )
-    (ensures (store_mem_aux (TBase TUInt128) addr ps v h0 == buffer_write b i v h0)) =
-    match ps with
-    | [] -> ()
-    | a::q ->
-      if valid_buffer (TBase TUInt128) addr a h0 then begin
-        let a:buffer128 = a in
-        BV.length_eq (BV.mk_buffer_view a uint128_view);
-        BV.get_view_mk_buffer_view a uint128_view;
-        BV.as_buffer_mk_buffer_view a uint128_view;
-        BV.length_eq (BV.mk_buffer_view b uint128_view);
-        BV.get_view_mk_buffer_view b uint128_view;
-        BV.as_buffer_mk_buffer_view b uint128_view;
+  match find_valid_buffer TUInt128 addr h with
+  | None -> ()
+  | Some a ->
+    BV.length_eq (BV.mk_buffer_view a uint128_view);
+    BV.get_view_mk_buffer_view a uint128_view;
+    BV.as_buffer_mk_buffer_view a uint128_view;
+    BV.length_eq (BV.mk_buffer_view b uint128_view);
+    BV.get_view_mk_buffer_view b uint128_view;
+    BV.as_buffer_mk_buffer_view b uint128_view;
+    assert (I.disjoint_or_eq a b);
+    assert (a == b)
 
-        assert (I.disjoint_or_eq a b);
-        assert (a == b);
-          ()
-      end
-      else begin
-        assert (b =!= a);
-          aux q h0
-      end
-  in aux h.ptrs h
-
-let rec same_get_addr_ptr (t:typ)
-                        (ptr:int)
-                        (h:mem)
-                        (ps:list b8{valid_mem_aux t ptr ps h})
-                        (b:buffer t{List.memP b h.ptrs})
-                        (i:nat{i < buffer_length b})
-                        (v:(type_of_typ t)) : Lemma
-  (let h1 = buffer_write b i v h in
-  get_addr_ptr t ptr h ps == get_addr_ptr t ptr h1 ps) =
-  match ps with
-  | a::q -> if valid_buffer t ptr a h then () else same_get_addr_ptr t ptr h q b i v
-
+let same_get_addr_ptr (t:base_typ)
+                      (ptr:int)
+                      (h:mem{valid_mem t ptr h})
+                      (b:buffer t{List.memP b h.ptrs})
+                      (i:nat{i < buffer_length b})
+                      (v:base_typ_as_vale_type t)
+  : Lemma (let h1 = buffer_write b i v h in
+           get_addr_ptr t ptr h == get_addr_ptr t ptr h1)
+  = let h1 = buffer_write b i v h in
+    assert (h.ptrs == h1.ptrs);
+    find_valid_buffer_ps t ptr h h1
+#reset-options "--z3rlimit_factor 2"
 let lemma_store_load_mem64 ptr v h =
-  let t = TBase TUInt64 in
+  let t = TUInt64 in
   let h1 = store_mem64 ptr v h in
-  store_buffer_write t ptr v h h.ptrs;
-  load_buffer_read t ptr h1 h1.ptrs;
-  let b = get_addr_ptr t ptr h h.ptrs in
+  store_buffer_write t ptr v h;
+  load_buffer_read t ptr h1;
+  let b = get_addr_ptr t ptr h in
   length_t_eq t b;
   let i = get_addr_in_ptr t (buffer_length b) (buffer_addr b h) ptr 0 in
-  same_get_addr_ptr t ptr h h.ptrs b i v;
+  same_get_addr_ptr t ptr h b i v;
   BV.as_buffer_mk_buffer_view b (uint_view t);
-  BV.as_seq_sel h1.hs (BV.mk_buffer_view b (uint_view t)) i;
-  ()
+  BV.as_seq_sel h1.hs (BV.mk_buffer_view b (uint_view t)) i
 
-#set-options "--z3rlimit 50"
 
-val different_addr_ptr64 (i:int) (i':nat{i <> i'})
-                       (h:mem{valid_mem_aux (TBase TUInt64) i h.ptrs h /\ valid_mem_aux (TBase TUInt64) i' h.ptrs h}) : Lemma
-  (let t = TBase TUInt64 in
-  get_addr_ptr t i h h.ptrs =!= get_addr_ptr t i' h h.ptrs \/
-    (let (b:buffer t) = get_addr_ptr t i h h.ptrs in
-     let (b':buffer t) = get_addr_ptr t i' h h.ptrs in
-     b == b' /\ get_addr_in_ptr t (buffer_length b) (buffer_addr b h) i 0 <>
+let rec different_addr_in_ptr
+          (t:base_typ) (n base:nat) (addr1 addr2:nat)
+          (i:nat)
+  : Lemma
+      (ensures (addr1 <> addr2 /\
+                valid_offset t n base addr1 i /\
+                valid_offset t n base addr2 i ==>
+                get_addr_in_ptr t n base addr1 i <> get_addr_in_ptr t n base addr2 i))
+      (decreases %[n-i])
+  = if (base + (view_n t) * i = addr1) || (base + (view_n t) * i = addr2) || i >= n then ()
+    else different_addr_in_ptr t n base addr1 addr2 (i+1)
+
+val different_addr_ptr64
+      (i:int)
+      (i':nat{i <> i'})
+      (h:mem{valid_mem TUInt64 i h /\ valid_mem TUInt64 i' h})
+ : Lemma
+     (let t = TUInt64 in
+      get_addr_ptr t i h =!= get_addr_ptr t i' h \/
+     (let b = get_addr_ptr t i h in
+      let b' = get_addr_ptr t i' h in
+      b == b' /\
+      get_addr_in_ptr t (buffer_length b) (buffer_addr b h) i 0 <>
       get_addr_in_ptr t (buffer_length b) (buffer_addr b h) i' 0))
 
-let rec different_addr_in_ptr (t:typ) (n base:nat) (addr1 addr2:nat) (i:nat{
-  (exists j. i <= j /\ j < n /\ base + (view_n t) `op_Multiply` j == addr1) /\
-  (exists k. i <= k /\ k < n /\ base + (view_n t) `op_Multiply` k == addr2)}) : Lemma
-  (requires addr1 <> addr2)
-  (ensures get_addr_in_ptr t n base addr1 i <> get_addr_in_ptr t n base addr2 i)
-  (decreases %[n-i]) =
-   if (base + (view_n t) `op_Multiply` i = addr1) || (base + (view_n t) `op_Multiply` i = addr2) || i >= n then ()
-   else different_addr_in_ptr t n base addr1 addr2 (i+1)
-
 let different_addr_ptr64 i i' h =
-  let t = TBase TUInt64 in
-  let rec aux (ps:list b8{valid_mem_aux t i ps h /\ valid_mem_aux t i' ps h}) :
-    Lemma (get_addr_ptr t i h ps =!= get_addr_ptr t i' h ps \/
-    (let b = get_addr_ptr t i h ps in
-     let b' = get_addr_ptr t i' h ps in
-     b == b' /\ get_addr_in_ptr t (buffer_length b) (buffer_addr b h) i 0 <>
-      get_addr_in_ptr t (buffer_length b) (buffer_addr b h) i' 0)) =
-     match ps with
-     | a::q -> if valid_buffer t i a h then begin
-       if valid_buffer t i' a h then begin
-         let a:buffer t = a in
-         assert (get_addr_ptr t i h ps == a);
-         assert (get_addr_ptr t i' h ps == a);
-         length_t_eq t a;
-         different_addr_in_ptr t (buffer_length a) (buffer_addr a h) i i' 0
-       end
-       else ()
-       end else if valid_buffer t i' a h then ()
-       else aux q
-  in aux h.ptrs
+  let t = TUInt64 in
+  match find_valid_buffer t i h, find_valid_buffer t i' h with
+  | Some b, Some b' ->
+    different_addr_in_ptr t (buffer_length b) (buffer_addr b h) i i' 0
+  | _ -> ()
 
+#set-options "--max_fuel 0 --max_ifuel 0 --z3rlimit_factor 4"
 let lemma_frame_store_mem64 ptr v h =
   let h1 = store_mem64 ptr v h in
-  let t = TBase TUInt64 in
+  let t = TUInt64 in
   let aux i' : Lemma
     (requires i' <> ptr /\ valid_mem64 ptr h /\ valid_mem64 i' h)
     (ensures load_mem64 i' h == load_mem64 i' h1) =
-    store_buffer_write t ptr v h h.ptrs;
-    load_buffer_read t i' h1 h1.ptrs;
-    load_buffer_read t i' h h.ptrs;
-    let b1 = get_addr_ptr t ptr h h.ptrs in
+    store_buffer_write t ptr v h;
+    load_buffer_read t i' h1;
+    load_buffer_read t i' h;
+    let b1 = get_addr_ptr t ptr h in
     let i1 = get_addr_in_ptr t (buffer_length b1) (buffer_addr b1 h) ptr 0 in
-    let b2 = get_addr_ptr t i' h h.ptrs in
+    let b2 = get_addr_ptr t i' h in
     let i2 = get_addr_in_ptr t (buffer_length b2) (buffer_addr b2 h) i' 0 in
-    same_get_addr_ptr t i' h h.ptrs b1 i1 v;
+    same_get_addr_ptr t i' h b1 i1 v;
     BV.as_buffer_mk_buffer_view b1 uint64_view;
     BV.upd_modifies h.hs (BV.mk_buffer_view b1 uint64_view) i1 (v_of_typ t v);
     assert (load_mem64 i' h == buffer_read b2 i2 h);
@@ -669,63 +596,51 @@ let lemma_frame_store_mem64 ptr v h =
 let lemma_valid_store_mem64 i v h = ()
 
 let lemma_store_load_mem128 ptr v h =
-  let t = TBase TUInt128 in
+  let t = TUInt128 in
   let h1 = store_mem128 ptr v h in
-  store_buffer_write t ptr v h h.ptrs;
-  load_buffer_read t ptr h1 h1.ptrs;
-  let b = get_addr_ptr t ptr h h.ptrs in
+  store_buffer_write t ptr v h;
+  load_buffer_read t ptr h1;
+  let b = get_addr_ptr t ptr h in
   length_t_eq t b;
   let i = get_addr_in_ptr t (buffer_length b) (buffer_addr b h) ptr 0 in
-  same_get_addr_ptr t ptr h h.ptrs b i v;
+  same_get_addr_ptr t ptr h b i v;
   BV.as_buffer_mk_buffer_view b (uint_view t);
   BV.as_seq_sel h1.hs (BV.mk_buffer_view b (uint_view t)) i;
   ()
 
-val different_addr_ptr128 (i:int) (i':nat{i <> i'})
-                       (h:mem{valid_mem_aux (TBase TUInt128) i h.ptrs h /\ valid_mem_aux (TBase TUInt128) i' h.ptrs h}) : Lemma
-  (let t = TBase TUInt128 in
-  get_addr_ptr t i h h.ptrs =!= get_addr_ptr t i' h h.ptrs \/
-    (let (b:buffer t) = get_addr_ptr t i h h.ptrs in
-     let (b':buffer t) = get_addr_ptr t i' h h.ptrs in
-     b == b' /\ get_addr_in_ptr t (buffer_length b) (buffer_addr b h) i 0 <>
+val different_addr_ptr128
+      (i:int)
+      (i':nat{i <> i'})
+      (h:mem{valid_mem TUInt128 i h /\ valid_mem TUInt128 i' h})
+ : Lemma
+     (let t = TUInt128 in
+      get_addr_ptr t i h =!= get_addr_ptr t i' h \/
+     (let b = get_addr_ptr t i h in
+      let b' = get_addr_ptr t i' h in
+      b == b' /\
+      get_addr_in_ptr t (buffer_length b) (buffer_addr b h) i 0 <>
       get_addr_in_ptr t (buffer_length b) (buffer_addr b h) i' 0))
-
 let different_addr_ptr128 i i' h =
-  let t = TBase TUInt128 in
-  let rec aux (ps:list b8{valid_mem_aux t i ps h /\ valid_mem_aux t i' ps h}) :
-    Lemma (get_addr_ptr t i h ps =!= get_addr_ptr t i' h ps \/
-    (let b = get_addr_ptr t i h ps in
-     let b' = get_addr_ptr t i' h ps in
-     b == b' /\ get_addr_in_ptr t (buffer_length b) (buffer_addr b h) i 0 <>
-      get_addr_in_ptr t (buffer_length b) (buffer_addr b h) i' 0)) =
-     match ps with
-     | a::q -> if valid_buffer t i a h then begin
-       if valid_buffer t i' a h then begin
-         let a:buffer t = a in
-         assert (get_addr_ptr t i h ps == a);
-         assert (get_addr_ptr t i' h ps == a);
-         length_t_eq t a;
-         different_addr_in_ptr t (buffer_length a) (buffer_addr a h) i i' 0
-       end
-       else ()
-       end else if valid_buffer t i' a h then ()
-       else aux q
-  in aux h.ptrs
+  let t = TUInt128 in
+  match find_valid_buffer t i h, find_valid_buffer t i' h with
+  | Some b, Some b' ->
+    different_addr_in_ptr t (buffer_length b) (buffer_addr b h) i i' 0
+  | _ -> ()
 
 let lemma_frame_store_mem128 ptr v h =
   let h1 = store_mem128 ptr v h in
-  let t = TBase TUInt128 in
+  let t = TUInt128 in
   let aux i' : Lemma
     (requires i' <> ptr /\ valid_mem128 ptr h /\ valid_mem128 i' h)
     (ensures load_mem128 i' h == load_mem128 i' h1) =
-    store_buffer_write t ptr v h h.ptrs;
-    load_buffer_read t i' h1 h1.ptrs;
-    load_buffer_read t i' h h.ptrs;
-    let b1 = get_addr_ptr t ptr h h.ptrs in
+    store_buffer_write t ptr v h;
+    load_buffer_read t i' h1;
+    load_buffer_read t i' h;
+    let b1 = get_addr_ptr t ptr h in
     let i1 = get_addr_in_ptr t (buffer_length b1) (buffer_addr b1 h) ptr 0 in
-    let b2 = get_addr_ptr t i' h h.ptrs in
+    let b2 = get_addr_ptr t i' h in
     let i2 = get_addr_in_ptr t (buffer_length b2) (buffer_addr b2 h) i' 0 in
-    same_get_addr_ptr t i' h h.ptrs b1 i1 v;
+    same_get_addr_ptr t i' h b1 i1 v;
     BV.as_buffer_mk_buffer_view b1 uint128_view;
     BV.upd_modifies h.hs (BV.mk_buffer_view b1 uint128_view) i1 (v_of_typ t v);
     assert (load_mem128 i' h == buffer_read b2 i2 h);
@@ -749,7 +664,7 @@ let lemma_frame_store_mem128 ptr v h =
 
 let lemma_valid_store_mem128 ptr v h = ()
 
-#set-options "--z3rlimit 100"
+//#set-options "--z3rlimit 100"
 
 val heap_shift (m1 m2:S.heap) (base:int) (n:nat) : Lemma
   (requires (forall i. 0 <= i /\ i < n ==> m1.[base + i] == m2.[base + i]))
@@ -759,26 +674,14 @@ let heap_shift m1 m2 base n =
   assert (forall i. base <= i /\ i < base + n ==>
     m1.[base + (i - base)] == m2.[base + (i - base)])
 
-val same_mem_get_heap_val64 (b:buffer64)
-                          (i:nat{i < buffer_length b})
-                          (v:nat64)
-                          (k:nat{k < buffer_length b})
-                          (h1:mem{List.memP b h1.ptrs})
-                          (h2:mem{h2 == buffer_write b i v h1})
-                          (mem1:S.heap{I.correct_down_p h1.hs h1.addrs mem1 b})
-                          (mem2:S.heap{I.correct_down_p h2.hs h2.addrs mem2 b}) : Lemma
-  (requires (Seq.index (buffer_as_seq h1 b) k == Seq.index (buffer_as_seq h2 b) k))
-  (ensures (let ptr = buffer_addr b h1 + 8 `op_Multiply` k in
-    forall i. {:pattern (mem1.[ptr+i])} i >= 0 /\ i < 8 ==> mem1.[ptr+i] == mem2.[ptr+i]))
-
 val same_mem_eq_slices64 (b:buffer64)
                        (i:nat{i < buffer_length b})
                        (v:nat64)
                        (k:nat{k < buffer_length b})
                        (h1:mem{List.memP b h1.ptrs})
                        (h2:mem{h2 == buffer_write b i v h1})
-                       (mem1:S.heap{I.correct_down_p h1.hs h1.addrs mem1 b})
-                       (mem2:S.heap{I.correct_down_p h2.hs h2.addrs mem2 b}) : Lemma
+                       (mem1:S.heap{IB.correct_down_p h1 mem1 b})
+                       (mem2:S.heap{IB.correct_down_p h2 mem2 b}) : Lemma
   (requires (Seq.index (buffer_as_seq h1 b) k == Seq.index (buffer_as_seq h2 b) k))
   (ensures (let open FStar.Mul in
     k * 8 + 8 <= B.length b /\
@@ -786,7 +689,7 @@ val same_mem_eq_slices64 (b:buffer64)
     Seq.slice (B.as_seq h2.hs b) (k * 8) (k * 8 + 8)))
 
 let same_mem_eq_slices64 b i v k h1 h2 mem1 mem2 =
-    let t = TBase TUInt64 in
+    let t = TUInt64 in
     BV.as_seq_sel h1.hs (BV.mk_buffer_view b (uint_view t)) k;
     BV.as_seq_sel h2.hs (BV.mk_buffer_view b (uint_view t)) k;
     BV.put_sel h1.hs (BV.mk_buffer_view b (uint_view t)) k;
@@ -796,20 +699,31 @@ let same_mem_eq_slices64 b i v k h1 h2 mem1 mem2 =
     BV.view_indexing (BV.mk_buffer_view b (uint_view t)) k;
     BV.length_eq (BV.mk_buffer_view b (uint_view t))
 
-#set-options "--z3rlimit 150"
 
 let length_up64 (b:buffer64) (h:mem) (k:nat{k < buffer_length b}) (i:nat{i < 8}) : Lemma
-  (8 `op_Multiply` k + i <= B.length b) =
+  (8 * k + i <= B.length b) =
   let vb = BV.mk_buffer_view b uint64_view in
   BV.length_eq vb;
   BV.as_buffer_mk_buffer_view b uint64_view;
   BV.get_view_mk_buffer_view b uint64_view;
   ()
 
+val same_mem_get_heap_val64 (b:buffer64)
+                          (i:nat{i < buffer_length b})
+                          (v:nat64)
+                          (k:nat{k < buffer_length b})
+                          (h1:mem{List.memP b h1.ptrs})
+                          (h2:mem{h2 == buffer_write b i v h1})
+                          (mem1:S.heap{IB.correct_down_p h1 mem1 b})
+                          (mem2:S.heap{IB.correct_down_p h2 mem2 b}) : Lemma
+  (requires (Seq.index (buffer_as_seq h1 b) k == Seq.index (buffer_as_seq h2 b) k))
+  (ensures (let ptr = buffer_addr b h1 + 8 * k in
+    forall i. {:pattern (mem1.[ptr+i])} i >= 0 /\ i < 8 ==> mem1.[ptr+i] == mem2.[ptr+i]))
+
 let same_mem_get_heap_val64 b j v k h1 h2 mem1 mem2 =
-  let ptr = buffer_addr b h1 + 8 `op_Multiply` k in
+  let ptr = buffer_addr b h1 + 8 * k in
   let addr = buffer_addr b h1 in
-  let aux (i:nat{i < 8}) : Lemma (mem1.[addr+(8 `op_Multiply` k + i)] == mem2.[addr+(8 `op_Multiply` k +i)]) =
+  let aux (i:nat{i < 8}) : Lemma (mem1.[addr+(8 * k + i)] == mem2.[addr+(8 * k +i)]) =
     BV.as_seq_sel h1.hs (BV.mk_buffer_view b uint64_view) k;
     BV.as_seq_sel h2.hs (BV.mk_buffer_view b uint64_view) k;
     same_mem_eq_slices64 b j v k h1 h2 mem1 mem2;
@@ -825,212 +739,216 @@ let same_mem_get_heap_val64 b j v k h1 h2 mem1 mem2 =
     ()
   in
   Classical.forall_intro aux;
-  assert (forall i. addr + (8 `op_Multiply` k + i) == ptr + i);
+  assert (forall i. addr + (8 * k + i) == ptr + i);
   ()
 
 let rec written_buffer_down64_aux1 (b:buffer64) (i:nat{i < buffer_length b}) (v:nat64)
-      (ps:list b8{I.list_disjoint_or_eq ps /\ List.memP b ps})
-      (h:mem{forall x. List.memP x ps ==> List.memP x h.ptrs})
+      (h:mem{List.memP b h.ptrs})
       (base:nat{base == buffer_addr b h})
       (k:nat) (h1:mem{h1 == buffer_write b i v h})
-      (mem1:S.heap{I.correct_down h.hs h.addrs ps mem1})
-      (mem2:S.heap{
-      (I.correct_down h1.hs h.addrs ps mem2) /\
-      (forall j. base <= j /\ j < base + k `op_Multiply` 8 ==> mem1.[j] == mem2.[j])}) :
-      Lemma (requires True)
-      (ensures (forall j. j >= base /\ j < base + 8 `op_Multiply` i ==> mem1.[j] == mem2.[j]))
+      (mem1:S.heap{IB.correct_down h mem1})
+      (mem2:S.heap{IB.correct_down h1 mem2 /\
+                   (forall j.{:pattern (mem1.[j]) \/ (mem2.[j])}
+                     base <= j /\ j < base + k * 8 ==>
+                     mem1.[j] == mem2.[j])})
+  : Lemma
+      (ensures (forall j. {:pattern (mem1.[j]) \/ (mem1.[j])}
+                  j >= base /\ j < base + 8 * i ==>
+                  mem1.[j] == mem2.[j]))
       (decreases %[i-k]) =
     if k >= i then ()
     else begin
-      let ptr = base + 8 `op_Multiply` k in
+      let ptr = base + 8 * k in
       same_mem_get_heap_val64 b i v k h h1 mem1 mem2;
       heap_shift mem1 mem2 ptr 8;
-      written_buffer_down64_aux1 b i v ps h base (k+1) h1 mem1 mem2
+      written_buffer_down64_aux1 b i v h base (k+1) h1 mem1 mem2
     end
 
 let rec written_buffer_down64_aux2 (b:buffer64) (i:nat{i < buffer_length b}) (v:nat64)
-      (ps:list b8{I.list_disjoint_or_eq ps /\ List.memP b ps})
-      (h:mem{forall x. List.memP x ps ==> List.memP x h.ptrs})
+      (h:mem{List.memP b h.ptrs})
       (base:nat{base == buffer_addr b h})
       (n:nat{n == buffer_length b})
       (k:nat{k > i}) (h1:mem{h1 == buffer_write b i v h})
-      (mem1:S.heap{I.correct_down h.hs h.addrs ps mem1})
-      (mem2:S.heap{
-      (I.correct_down h1.hs h.addrs ps mem2) /\
-      (forall j. base + 8 `op_Multiply` (i+1) <= j /\ j < base + k `op_Multiply` 8 ==>
-      mem1.[j] == mem2.[j])}) :
-      Lemma
-      (requires True)
-      (ensures (forall j. j >= base + 8 `op_Multiply` (i+1) /\ j < base + 8 `op_Multiply` n ==>
-        mem1.[j] == mem2.[j]))
+      (mem1:S.heap{IB.correct_down h mem1})
+      (mem2:S.heap{IB.correct_down h1 mem2 /\
+                   (forall j. {:pattern (mem1.[j]) \/ (mem2.[j])}
+                     base + 8 * (i+1) <= j /\ j < base + k * 8 ==>
+                     mem1.[j] == mem2.[j])})
+  : Lemma
+      (ensures (forall j. {:pattern (mem1.[j]) \/ (mem2.[j])}
+                     j >= base + 8 * (i+1) /\ j < base + 8 * n ==>
+                     mem1.[j] == mem2.[j]))
       (decreases %[n-k]) =
     if k >= n then ()
     else begin
-      let ptr = base + 8 `op_Multiply` k in
+      let ptr = base + 8 * k in
       same_mem_get_heap_val64 b i v k h h1 mem1 mem2;
       heap_shift mem1 mem2 ptr 8;
-      written_buffer_down64_aux2 b i v ps h base n (k+1) h1 mem1 mem2
+      written_buffer_down64_aux2 b i v h base n (k+1) h1 mem1 mem2
     end
 
-let written_buffer_down64 (b:buffer64) (i:nat{i < buffer_length b}) (v:nat64)
-  (ps: list b8{I.list_disjoint_or_eq ps /\ List.memP b ps}) (h:mem{forall x. List.memP x ps ==> List.memP x h.ptrs}) :
-  Lemma (
-    let mem1 = I.down_mem h.hs h.addrs ps in
+let written_buffer_down64 (b:buffer64) (i:nat{i < buffer_length b}) (v:nat64) (h:mem)
+  : Lemma
+      (requires List.memP b h.ptrs)
+      (ensures (
+          let mem1 = I.down_mem h in
+          let h1 = buffer_write b i v h in
+          let mem2 = I.down_mem h1 in
+          let base = buffer_addr b h in
+          let n = buffer_length b in
+          forall j. {:pattern (mem1.[j]) \/ (mem2.[j])}
+               (base <= j /\ j < base + 8 * i) \/
+               (base + 8 * (i+1) <= j /\ j < base + 8 * n) ==>
+               mem1.[j] == mem2.[j]))
+  = let mem1 = I.down_mem h in
     let h1 = buffer_write b i v h in
-    let mem2 = I.down_mem h1.hs h.addrs ps in
+    let mem2 = I.down_mem h1 in
     let base = buffer_addr b h in
     let n = buffer_length b in
-    forall j. (base <= j /\ j < base + 8 `op_Multiply` i) \/
-         (base + 8 `op_Multiply` (i+1) <= j /\ j < base + 8 `op_Multiply` n) ==>
-         mem1.[j] == mem2.[j]) =
-    let mem1 = I.down_mem h.hs h.addrs ps in
-    let h1 = buffer_write b i v h in
-    let mem2 = I.down_mem h1.hs h.addrs ps in
-    let base = buffer_addr b h in
-    let n = buffer_length b in
-    written_buffer_down64_aux1 b i v ps h base 0 h1 mem1 mem2;
-    written_buffer_down64_aux2 b i v ps h base n (i+1) h1 mem1 mem2
+    written_buffer_down64_aux1 b i v h base 0 h1 mem1 mem2;
+    written_buffer_down64_aux2 b i v h base n (i+1) h1 mem1 mem2
 
-#set-options "--z3rlimit 50"
-
-let unwritten_buffer_down_aux (t:typ) (b:buffer t) (i:nat{i < buffer_length b}) (v:type_of_typ t)
-  (ps: list b8{I.list_disjoint_or_eq ps /\ List.memP b ps})
-  (h:mem{forall x. List.memP x ps ==> List.memP x h.ptrs})
-  (a:b8{a =!= b /\ List.memP a ps})  :
-  Lemma (let base = h.addrs a in
-    let mem1 = I.down_mem h.hs h.addrs ps in
-    let h1 = buffer_write b i v h in
-    let mem2 = I.down_mem h1.hs h.addrs ps in
-    forall j. j >= base /\ j < base + B.length a ==> mem1.[j] == mem2.[j]) =
-    if B.length a = 0 then ()
-    else
-    let mem1 = I.down_mem h.hs h.addrs ps in
-    let h1 = buffer_write b i v h in
-    let mem2 = I.down_mem h1.hs h.addrs ps in
-    let base = h.addrs a in
-    let s0 = B.as_seq h.hs a in
-    let s1 = B.as_seq h1.hs a in
-    assert (B.disjoint a b);
-    heap_shift mem1 mem2 base (B.length a)
-
-let unwritten_buffer_down (t:typ) (b:buffer t) (i:nat{i < buffer_length b}) (v:type_of_typ t)
-  (ps: list b8{I.list_disjoint_or_eq ps /\ List.memP b ps})
-  (h:mem{forall x. List.memP x ps ==> List.memP x h.ptrs}) : Lemma (
-    let mem1 = I.down_mem h.hs h.addrs ps in
-    let h1 = buffer_write b i v h in
-    let mem2 = I.down_mem h1.hs h.addrs ps in
-    forall  (a:b8{List.memP a ps /\ a =!= b}) j.
-    let base = h.addrs a in
-    j >= base /\ j < base + B.length a ==> mem1.[j] == mem2.[j]) =
-    let mem1 = I.down_mem h.hs h.addrs ps in
-    let h1 = buffer_write b i v h in
-    let mem2 = I.down_mem h1.hs h.addrs ps in
-    let fintro (a:b8{List.memP a ps /\ a =!= b})
+let unwritten_buffer_down (t:base_typ) (b:buffer t)
+                          (i:nat{i < buffer_length b})
+                          (v:base_typ_as_vale_type t)
+                          (h:mem{List.memP b h.ptrs})
+  : Lemma
+      (ensures (
+        let mem1 = I.down_mem h in
+        let h1 = buffer_write b i v h in
+        let mem2 = I.down_mem h1 in
+        forall  (a:b8{List.memP a h.ptrs /\ a =!= b}) j. {:pattern mem1.[j]; List.memP a h.ptrs \/ mem2.[j]; List.memP a h.ptrs}
+          let base = h.addrs a in
+          j >= base /\ j < base + B.length a ==> mem1.[j] == mem2.[j]))
+  = let aux (a:b8{a =!= b /\ List.memP a h.ptrs})
       : Lemma
-      (forall j. let base = h.addrs a in
-      j >= base /\ j < base + B.length a ==>
-        mem1.[j] == mem2.[j]) =
-      let base = h.addrs a in
-      unwritten_buffer_down_aux t b i v ps h a
+        (ensures (
+          let base = h.addrs a in
+          let mem1 = I.down_mem h in
+          let h1 = buffer_write b i v h in
+          let mem2 = I.down_mem h1 in
+          forall j.
+            j >= base /\ j < base + B.length a ==>
+            mem1.[j] == mem2.[j]))
+      = if B.length a = 0 then ()
+        else
+          let mem1 = I.down_mem h in
+          let h1 = buffer_write b i v h in
+          let mem2 = I.down_mem h1 in
+          let base = h.addrs a in
+          let s0 = B.as_seq h.hs a in
+          let s1 = B.as_seq h1.hs a in
+          assert (B.disjoint a b);
+          assert (Seq.equal s0 s1);
+          assert (forall (i:nat). {:pattern (mem1.[base + i])}
+                    i < Seq.length s0 ==> v_to_typ TUInt8 (Seq.index s0 i) == mem1.[base + i]);
+          heap_shift mem1 mem2 base (B.length a)
     in
-    Classical.forall_intro fintro
+    Classical.forall_intro aux
 
 let store_buffer_down64_mem (b:buffer64) (i:nat{i < buffer_length b}) (v:nat64)
-  (ps: list b8{I.list_disjoint_or_eq ps /\ List.memP b ps})
-  (h:mem{forall x. List.memP x ps ==> List.memP x h.ptrs}) :
-  Lemma (
-    let mem1 = I.down_mem h.hs h.addrs ps in
+                            (h:mem{List.memP b h.ptrs})
+  : Lemma
+      (ensures (
+        let mem1 = I.down_mem h in
+        let h1 = buffer_write b i v h in
+        let mem2 = I.down_mem h1 in
+        let base = buffer_addr b h in
+        forall (j:int). {:pattern mem1.[j] \/ mem2.[j]}
+          j < base + 8 * i \/ j >= base + 8 * (i+1) ==>
+          mem1.[j] == mem2.[j]))
+  = let mem1 = I.down_mem h in
     let h1 = buffer_write b i v h in
-    let mem2 = I.down_mem h1.hs h.addrs ps in
-    let base = buffer_addr b h in
-    forall (j:int). j < base + 8 `op_Multiply` i \/ j >= base + 8 `op_Multiply` (i+1) ==>
-      mem1.[j] == mem2.[j]) =
-    let mem1 = I.down_mem h.hs h.addrs ps in
-    let h1 = buffer_write b i v h in
-    let mem2 = I.down_mem h1.hs h.addrs ps in
+    let mem2 = I.down_mem h1 in
     let base = buffer_addr b h in
     let n = buffer_length b in
-    let aux (j:int) : Lemma
-      (j < base + 8 `op_Multiply` i \/ j >= base + 8 `op_Multiply` (i+1) ==>
-      mem1.[j] == mem2.[j]) =
-        if j >= base && j < base + B.length b then begin
-          written_buffer_down64 b i v ps h;
-          length_t_eq (TBase TUInt64) b
+    let aux (j:int)
+      : Lemma
+          (j < base + 8 * i \/ j >= base + 8 * (i+1) ==>
+           mem1.[j] == mem2.[j])
+      = if j >= base && j < base + B.length b then begin
+          written_buffer_down64 b i v h;
+          length_t_eq (TUInt64) b
         end
-        else (
-        unwritten_buffer_down (TBase TUInt64) b i v ps h;
-        I.same_unspecified_down h.hs h1.hs h.addrs ps;
-        ()
-        )
-    in Classical.forall_intro aux
+        else if not (I.valid_addr h j)
+        then I.same_unspecified_down h.hs h1.hs h.ptrs
+        else unwritten_buffer_down TUInt64 b i v h
+    in
+    Classical.forall_intro aux
 
-let store_buffer_aux_down64_mem (ptr:int) (v:nat64) (h:mem{valid_mem64 ptr h}) : Lemma (
-  let mem1 = I.down_mem h.hs h.addrs h.ptrs in
-  let h1 = store_mem_aux (TBase TUInt64) ptr h.ptrs v h in
-  let mem2 = I.down_mem h1.hs h.addrs h.ptrs in
-  forall j. j < ptr \/ j >= ptr + 8 ==> mem1.[j] == mem2.[j]) =
-  let t = TBase TUInt64 in
-  let h1 = store_mem_aux t ptr h.ptrs v h in
-  let b = get_addr_ptr t ptr h h.ptrs in
-  length_t_eq t b;
-  let i = get_addr_in_ptr t (buffer_length b) (buffer_addr b h) ptr 0 in
-  store_buffer_write t ptr v h h.ptrs;
-  assert (buffer_addr b h + 8 `op_Multiply` i == ptr);
-  assert (buffer_addr b h + 8 `op_Multiply` (i+1) == ptr + 8);
-  store_buffer_down64_mem b i v h.ptrs h
+let store_buffer_aux_down64_mem (ptr:int) (v:nat64) (h:mem{valid_mem64 ptr h})
+  : Lemma
+      (ensures (
+        let mem1 = I.down_mem h in
+        let h1 = store_mem (TUInt64) ptr v h in
+        let mem2 = I.down_mem h1 in
+        forall j. {:pattern mem1.[j] \/ mem2.[j]}
+          j < ptr \/ j >= ptr + 8 ==>
+          mem1.[j] == mem2.[j]))
+  = let t = TUInt64 in
+    let h1 = store_mem t ptr v h in
+    let b = get_addr_ptr t ptr h in
+    length_t_eq t b;
+    let i = get_addr_in_ptr t (buffer_length b) (buffer_addr b h) ptr 0 in
+    store_buffer_write t ptr v h;
+    assert (buffer_addr b h + 8 * i == ptr);
+    assert (buffer_addr b h + 8 * (i+1) == ptr + 8);
+    store_buffer_down64_mem b i v h
 
-let store_buffer_aux_down64_mem2 (ptr:int) (v:nat64) (h:mem{valid_mem64 ptr h}) : Lemma (
-  let h1 = store_mem_aux (TBase TUInt64) ptr h.ptrs v h in
-  let mem2 = I.down_mem h1.hs h.addrs h.ptrs in
-  S.get_heap_val64 ptr mem2 == v) =
-  let t = TBase TUInt64 in
-  let b = get_addr_ptr t ptr h h.ptrs in
-  length_t_eq t b;
-  let i = get_addr_in_ptr t (buffer_length b) (buffer_addr b h) ptr 0 in
-  let h1 = store_mem_aux t ptr h.ptrs v h in
-  let mem2 = I.down_mem h1.hs h.addrs h.ptrs in
-  store_buffer_write t ptr v h h.ptrs;
-  assert (Seq.index (buffer_as_seq h1 b) i == v);
-  index64_get_heap_val64 h1 b mem2 i;
-  ()
+let store_buffer_aux_down64_mem2 (ptr:int) (v:nat64) (h:mem{valid_mem64 ptr h})
+  : Lemma
+      (ensures (
+        let h1 = store_mem (TUInt64) ptr v h in
+        let mem2 = I.down_mem h1 in
+        S.get_heap_val64 ptr mem2 == v))
+  = let t = TUInt64 in
+    let b = get_addr_ptr t ptr h in
+    length_t_eq t b;
+    let i = get_addr_in_ptr t (buffer_length b) (buffer_addr b h) ptr 0 in
+    let h1 = store_mem t ptr v h in
+    let mem2 = I.down_mem h1 in
+    store_buffer_write t ptr v h;
+    assert (Seq.index (buffer_as_seq h1 b) i == v);
+    index64_get_heap_val64 h1 b mem2 i
 
-let in_bounds64 (h:mem) (b:buffer64) (i:nat{i < buffer_length b}) : Lemma
-  (forall j. j >= h.addrs b + 8 `op_Multiply` i /\ j < h.addrs b + 8 `op_Multiply` i + 8 ==>
-    j < h.addrs b + B.length b) =
-  length_t_eq (TBase TUInt64) b;
-  ()
+let in_bounds64 (h:mem) (b:buffer64) (i:nat{i < buffer_length b})
+  : Lemma
+      (ensures (forall j. h.addrs b + 8 * i <= j  /\
+                     j < h.addrs b + 8 * i + 8 ==>
+                     j < h.addrs b + B.length b))
+  = length_t_eq (TUInt64) b
 
 open X64.Machine_s
 
 let valid_taint_buf (b:b8) (mem:mem) (memTaint:memtaint) t =
   let addr = mem.addrs b in
-  (forall (i:nat{i < B.length b}). memTaint.[addr + i] = t)
+  (forall (i:nat{i < B.length b}).{:pattern (memTaint.[addr + i])} memTaint.[addr + i] = t)
 
 let valid_taint_buf64 b mem memTaint t = valid_taint_buf b mem memTaint t
 
 let valid_taint_buf128 b mem memTaint t = valid_taint_buf b mem memTaint t
 
 let lemma_valid_taint64 b memTaint mem i t =
-  length_t_eq (TBase TUInt64) b;
-  let ptr = buffer_addr b mem + 8 `op_Multiply` i in
+  length_t_eq (TUInt64) b;
+  let ptr = buffer_addr b mem + 8 * i in
   let aux i' : Lemma
     (requires i' >= ptr /\ i' < ptr + 8)
-    (ensures memTaint.[i'] == t) = 
-    assert (i' == mem.addrs b + (8 `op_Multiply` i + i' - ptr));
+    (ensures memTaint.[i'] == t) =
+    assert (i' == mem.addrs b + (8 * i + i' - ptr));
     () in
   Classical.forall_intro (Classical.move_requires aux)
 
 let lemma_valid_taint128 b memTaint mem i t =
-  length_t_eq (TBase TUInt128) b;
-  let ptr = buffer_addr b mem + 16 `op_Multiply` i in
+  length_t_eq (TUInt128) b;
+  let ptr = buffer_addr b mem + 16 * i in
   let aux i' : Lemma
     (requires i' >= ptr /\ i' < ptr + 16)
-    (ensures memTaint.[i'] == t) = 
-    assert (i' == mem.addrs b + (16 `op_Multiply` i + i' - ptr));
+    (ensures memTaint.[i'] == t) =
+    assert (i' == mem.addrs b + (16 * i + i' - ptr));
     () in
   Classical.forall_intro (Classical.move_requires aux)
 
-let same_memTaint (t:typ) (b:buffer t) (mem0 mem1:mem) (memT0 memT1:memtaint) : Lemma
+let same_memTaint (t:base_typ) (b:buffer t) (mem0 mem1:mem) (memT0 memT1:memtaint) : Lemma
   (requires modifies (loc_buffer b) mem0 mem1 /\
     (forall p. Map.sel memT0 p == Map.sel memT1 p))
   (ensures memT0 == memT1) =
@@ -1038,46 +956,47 @@ let same_memTaint (t:typ) (b:buffer t) (mem0 mem1:mem) (memT0 memT1:memtaint) : 
   ()
 
 let same_memTaint64 b mem0 mem1 memtaint0 memtaint1 =
-same_memTaint (TBase TUInt64) b mem0 mem1 memtaint0 memtaint1
+  same_memTaint (TUInt64) b mem0 mem1 memtaint0 memtaint1
 
 let same_memTaint128 b mem0 mem1 memtaint0 memtaint1 =
-  same_memTaint (TBase TUInt128) b mem0 mem1 memtaint0 memtaint1
+  same_memTaint (TUInt128) b mem0 mem1 memtaint0 memtaint1
 
 let modifies_valid_taint64 b p h h' memTaint t = ()
 let modifies_valid_taint128 b p h h' memTaint t = ()
 
 let valid_taint_bufs (mem:mem) (memTaint:memtaint) (ps:list b8) (ts:b8 -> GTot taint) =
-  forall b. List.memP b ps ==> valid_taint_buf b mem memTaint (ts b)
+  forall b.{:pattern List.memP b ps} List.memP b ps ==> valid_taint_buf b mem memTaint (ts b)
 
-val create_valid_memtaint
-  (mem:mem)
-  (ps:list b8{I.list_disjoint_or_eq ps})
-  (ts:b8 -> GTot taint) :
-  GTot (m:memtaint{valid_taint_bufs mem m ps ts})
+#set-options "--initial_fuel 1 --max_fuel 1 --initial_ifuel 1 --max_ifuel 1"
+let rec write_taint_lemma (i:nat) (mem:IB.mem) (ts:b8 -> GTot taint) (b:b8{i <= B.length b})
+                          (accu:memtaint{forall j. 0 <= j /\ j < i ==> accu.[mem.addrs b+j] = ts b})
+   : Lemma
+       (ensures (
+         let m = IB.write_taint i mem ts b accu in
+         let addr = mem.addrs b in
+         (forall j. {:pattern m.[addr+j]} 0 <= j /\ j < B.length b ==> m.[addr+j] = ts b) /\
+         (forall j. {:pattern m.[j]} j < addr \/ j >= addr + B.length b ==> m.[j] == accu.[j])))
+       (decreases %[B.length b - i])
+   = let m = IB.write_taint i mem ts b accu in
+     let addr = mem.addrs b in
+     if i >= B.length b then ()
+     else let new_accu = accu.[addr+i] <- ts b in
+          assert (IB.write_taint i mem ts b accu ==
+                  IB.write_taint (i + 1) mem ts b new_accu);
+          assert (Set.equal (Map.domain new_accu) (Set.complement Set.empty));
+          assert (forall j. 0 <= j /\ j < i + 1 ==> new_accu.[addr + i] == ts b);
+          write_taint_lemma (i + 1) mem ts b new_accu
 
-private
-let rec write_taint (t:taint) (length addr:nat) (i:nat{i <= length}) (accu:memtaint{
-  forall j. 0 <= j /\ j < i ==> accu.[addr+j] = t}) : Tot (m:memtaint{
-  forall j. (0 <= j /\ j < length ==> m.[addr+j] = t) /\
-       (j < addr \/ j >= addr + length ==> m.[j] == accu.[j])})
-  (decreases %[length - i]) =
-  if i >= length then accu
-  else (
-    let new_accu = accu.[addr+i] <- t in
-    assert (Set.equal (Map.domain new_accu) (Set.complement Set.empty));
-    write_taint t length addr (i+1) new_accu
-  )
-
-#set-options "--z3rlimit 128"
-
-let create_valid_memtaint mem ps ts =
-  let memTaint = FStar.Map.const Public in
-  assert (Set.equal (Map.domain memTaint) (Set.complement Set.empty));
-  let rec aux (ps:list b8{I.list_disjoint_or_eq ps}) (accu:memtaint) : GTot (m:memtaint{valid_taint_bufs mem m ps ts /\ (forall j. (forall b. List.memP b ps ==> j < mem.addrs b \/ j >= mem.addrs b + B.length b) ==> accu.[j] = m.[j])}) =
-  match ps with
-    | [] -> accu
-    | b::q ->
-    let accu = aux q (write_taint (ts b) (B.length b) (mem.addrs b) 0 accu) in
-    assert (forall p. List.memP p q ==> I.disjoint_or_eq p b);
-    accu
-  in aux ps memTaint
+let rec valid_memtaint (mem:mem) (ps:list b8{I.list_disjoint_or_eq ps}) (ts:b8 -> GTot taint)
+  : Lemma (valid_taint_bufs mem (IB.create_memtaint mem ps ts) ps ts)
+  = match ps with
+    | [] -> ()
+    | b :: q ->
+      assert (List.memP b ps);
+      assert (forall i. {:pattern List.memP i q} List.memP i q ==> List.memP i ps);
+      assert (I.list_disjoint_or_eq q);
+      valid_memtaint mem q ts;
+      assert (IB.create_memtaint mem ps ts ==
+              IB.write_taint 0 mem ts b (IB.create_memtaint mem q ts));
+      write_taint_lemma 0 mem ts b (IB.create_memtaint mem q ts);
+      assert (forall p. List.memP p q ==> I.disjoint_or_eq p b)
