vale/specs/interop/Interop.Types.fst
@@ -1,0 +1,34 @@
+module Interop.Types
+module B = LowStar.Buffer
+module W = Words_s
+module L = FStar.List.Tot
+
+let __reduce__ = ()
+
+type base_typ:eqtype =
+  | TUInt8
+  | TUInt16
+  | TUInt32
+  | TUInt64
+  | TUInt128
+
+[@__reduce__]
+let view_n = function
+  | TUInt8 -> 1
+  | TUInt16 -> 2
+  | TUInt32 -> 4
+  | TUInt64 -> 8
+  | TUInt128 -> 16
+
+let b8 = B.buffer UInt8.t
+
+let disjoint_addr addr1 length1 addr2 length2 =
+  (* The first buffer is completely before the second, or the opposite *)
+  addr1 + length1 < addr2 ||
+  addr2 + length2 < addr1
+
+type addr_map = m:(b8 -> W.nat64){
+  (forall (buf1 buf2:b8).{:pattern (m buf1); (m buf2)}
+    B.disjoint buf1 buf2 ==>
+    disjoint_addr (m buf1) (B.length buf1) (m buf2) (B.length buf2)) /\
+  (forall (b:b8).{:pattern (m b)} m b + B.length b < W.pow2_64)}
